Cas.lean
@@ -3,6 +3,7 @@ import Cas.Reduce
 import Cas.Bracket
 import Cas.Encode
 import Cas.Bin
+import Cas.Int
 import Cas.Expr
 import Cas.Algebra
 import Cas.Diff
